fstar/Hacspec.Lib.Seq.fst
@@ -4,15 +4,17 @@ module LSeq = Lib.Sequence
 
 open Hacspec.Lib.Int
 
-type lseq (a: Type) (len: uint_size) = LSeq.lseq a (v len)
+type lseq (a: Type) (len: uint_size) = LSeq.lseq a len
+
+type byte_seq (len: uint_size) = lseq uint8 len
 
 (**** Array manipulation *)
 
 assume val new_ (#a: Type) (len: uint_size) (_: unit) : lseq a len
 
-assume val array_index (#a: Type) (#len: uint_size) (s: lseq a len) (i: uint_size{UInt32.v i < UInt32.v len}) : a
+assume val array_index (#a: Type) (#len: uint_size) (s: lseq a len) (i: uint_size{i < len}) : a
 
-assume val array_upd (#a: Type) (#len: uint_size) (s: lseq a len) (i: uint_size{UInt32.v i < UInt32.v len})
+assume val array_upd (#a: Type) (#len: uint_size) (s: lseq a len) (i: uint_size{i < len})
  (new_v: a) : lseq a len
 
 assume val from_slice (#a: Type) (#len: uint_size) (input: lseq a len) (start: uint_size) (new_len: uint_size) : lseq a new_len
