fstar/Hacspec.Poly1305.fst
@@ -25,7 +25,7 @@ let encode_r (r_1864 : block) : field_element =
   let r_128_1865 = RSeq.from_slice (r_1864) (usize 0) (blocksize) in
   let r_uint_1866 = uint128_from_le_bytes (r_128_1865) in
   let r_uint_1867 =
-    r_uint_1866 & uint128 (pub_u128 0xffffffc0ffffffc0ffffffc0fffffff)
+    r_uint_1866 &. secret (pub_u128 0xffffffc0ffffffc0ffffffc0fffffff)
   in
   RNat.from_secret_literal (r_uint_1867)
 
@@ -37,8 +37,8 @@ let encode (block_1868 : byte_seq) : field_element =
   let w_elem_1871 =
     RNat.from_secret_literal (uint128_from_le_bytes (block_as_u128_1870))
   in
-  let l_elem_1872 = RNat.from_canvas (RSeq.pow2 (usize 8 * block_len_1869)) in
-  w_elem_1871 + l_elem_1872
+  let l_elem_1872 = RNat.from_canvas (RSeq.pow2 (usize 8 *. block_len_1869)) in
+  w_elem_1871 +. l_elem_1872
 
 let poly_inner (m_1873 : byte_seq) (r_1874 : field_element) : field_element =
   let acc_1875 = RNat.from_literal (pub_u128 0x0) in
@@ -46,7 +46,7 @@ let poly_inner (m_1873 : byte_seq) (r_1874 : field_element) : field_element =
     foldi (usize 0) (num_chunks (m_1873) (blocksize)) (fun (i_1876, (acc_1875)
       ) ->
       let (_, block_1877) = get_chunk (m_1873) (blocksize) (i_1876) in
-      let acc_1875 = acc_1875 + encode (block_1877) * r_1874 in
+      let acc_1875 = acc_1875 +. encode (block_1877) *. r_1874 in
       (acc_1875))
     (acc_1875)
   in
@@ -62,7 +62,7 @@ let poly (m_1878 : byte_seq) (key_1879 : key_poly) : tag =
     encode_r (RSeq.from_slice_range (key_1879) ((usize 0, blocksize)))
   in
   let a_1882 = poly_inner (m_1878) (r_elem_1881) in
-  let n_1883 = a_1882 + s_elem_1880 in
+  let n_1883 = a_1882 +. s_elem_1880 in
   let n_v_1884 = to_public_byte_seq_le (n_1883) in
   let tag_1885 = RSeq.new_ BLOCKSIZE () in
   let (tag_1885) =
